ironfleet/src/Dafny/Distributed/Impl/Raft/CTypes.i.dfy
@@ -17,16 +17,41 @@ function AbstractifyCClockReadingToClockReading(cclock:CClockReading) : ClockRea
   ClockReading(cclock.t as int)
 }
 
-datatype CLogEntry = CLogEntry(term:uint64, index:uint64, req:CAppRequest, is_commited:uint64)
+datatype CLogEntry = CLogEntry(term:uint64, index:uint64, req:CAppRequest, seqno:uint64, is_commited:uint64)
+
+// for `log` in server_impl
+function method ServerMaxLogSize() : int
+{
+  0xFFFF_FFFF_FFFF_FFFF
+}
+
+function method MaxLogEntryTerm() : int {
+  0xFFFF_FFFF_FFFF_FFFF
+}
+
+function method MaxLogEntryIndex() : int {
+  0xFFFF_FFFF_FFFF_FFFF
+}
+
+function method MaxSeqno() : int {
+  0xFFFF_FFFF_FFFF_FFFF
+}
 
 predicate method ValidLogEntry(entry:CLogEntry) {
-  && 0 < entry.term <= 0xFFFF_FFFF_FFFF_FFFF
-  && 0 < entry.index <= 0xFFFF_FFFF_FFFF_FFFF
+  && 0 <= entry.term <= MaxLogEntryTerm() as uint64
+  && 0 <= entry.index <= MaxLogEntryIndex() as uint64
+  && 0 <= entry.seqno <= MaxSeqno() as uint64
   && (entry.is_commited == 0 || entry.is_commited == 1)
   && CAppRequestMarshallable(entry.req)
 }
 
 function method LogEntrySeqSizeLimit() : int { 100 }
+
+predicate method LogEntrySeqIndexIncreasing(log:seq<CLogEntry>) 
+  requires forall i :: 0 <= i < |log| ==> ValidLogEntry(log[i])
+{
+  (forall i :: 0 <= i < |log|-1 && log[i].index > 0 ==> log[i].index as int + 1 == log[i+1].index as int)
+}
 
 predicate method ValidLogEntrySeq(entries:seq<CLogEntry>) {
   && (forall entry :: entry in entries ==> ValidLogEntry(entry))
@@ -43,7 +68,7 @@ predicate CLogEntrySeqIsAbstractable(log_entries:seq<CLogEntry>) {
 
 function AbstractifyCLogEntryToRaftLogEntry(entry:CLogEntry) : LogEntry
 {
-  LogEntry(entry.term as int, entry.index as int, AbstractifyCAppRequestToAppRequest(entry.req), entry.is_commited == 1)
+  LogEntry(entry.term as int, entry.index as int, AbstractifyCAppRequestToAppRequest(entry.req), entry.seqno as int, entry.is_commited == 1)
 }
 
 function AbstractifyCLogEntrySeqToRaftLogEntrySeq(entries:seq<CLogEntry>) : seq<LogEntry>
