ironfleet/src/Dafny/Distributed/Impl/Raft/ServerImpl.i.dfy
@@ -10,8 +10,12 @@ include "../../Protocol/Raft/Types.i.dfy"
 include "../../Services/Raft/AppStateMachine.s.dfy"
 include "../Common/GenericMarshalling.i.dfy"
 include "../Common/NetClient.i.dfy"
+include "AppInterface.i.dfy"
+include "CMessage.i.dfy"
 include "Config.i.dfy"
+include "CTypes.i.dfy"
 include "PacketParsing.i.dfy"
+
 
 module Raft__ServerImpl_i {
 
@@ -26,7 +30,10 @@ import opened Raft__Types_i
 import opened Common__GenericMarshalling_i
 import opened Common__NetClient_i
 import opened AppStateMachine_s
+import opened Raft__AppInterface_i
+import opened Raft__CMessage_i
 import opened Raft__ConfigState_i
+import opened Raft__CTypes_i
 import opened Raft__PacketParsing_i
 
 class ServerImpl
@@ -44,13 +51,13 @@ class ServerImpl
   var current_leader:Option<EndPoint>;
   var current_term:uint64;
   var voted_for:Option<EndPoint>;
-  var log:seq<LogEntry>;
+  var log:seq<CLogEntry>;
   // volatile state on all servers
   var commit_index:uint64;
   var last_applied:uint64;
   // volatile state on leaders
-  var next_index:map<EndPoint, int>;
-  var match_index:map<EndPoint, int>;
+  var next_index:map<EndPoint, uint64>;
+  var match_index:map<EndPoint, uint64>;
   var num_replicated:seq<int>; // log index -> num of replicated
 
   var msg_grammar:G;
@@ -91,10 +98,42 @@ class ServerImpl
     && repr == { this } + NetClientRepr(net_client)
     && msg_grammar == CMessage_grammar()
     && (current_leader.None? || (current_leader.Some? && current_leader.v in config.global_config.server_eps))
+    // Term
+    && current_term as int <= MaxLogEntryTerm()
+    // Log
+    && 1 <= |log| <= ServerMaxLogSize() as int
+    && log[0] == CLogEntry(0, 0, [], 0, 1)
+    && (forall i :: 0 <= i < |log| ==> ValidLogEntry(log[i]))
+    // TODO: this may not be true when truncating
+    && (forall i :: 0 <= i < |log| ==> log[i].index as int == i)
+    && LogEntrySeqIndexIncreasing(log)
+    && (
+      role.Leader? ==> (
+        forall ep :: ep in config.global_config.server_eps ==> (
+          && ep in next_index 
+          && ep in match_index
+          && 1 <= next_index[ep] <= |log| as uint64
+          && 0 <= match_index[ep] < next_index[ep]
+        )
+      )
+    )
+    && |config.global_config.server_eps| >= 1
+  }
+
+  function MapUint64MapValueToInt<T>(m:map<T, uint64>) : map<T, int>
+    requires true
+    ensures forall k :: k in m ==> k in MapUint64MapValueToInt(m)
+    ensures forall k, v :: k in m && v == m[k] ==> MapUint64MapValueToInt(m)[k] == v as int
+  {
+    map k:T | k in m :: m[k] as int
   }
 
   function AbstractifyToRaftServer() : RaftServer
     reads this
+    reads this.app_state
+    reads if net_client != null then NetClientIsValid.reads(net_client) else {}
+    requires Valid()
+    ensures Valid()
   {
     RaftServer(
       AbstractifyServerConfigStateToRaftServerConfig(config),
@@ -104,23 +143,71 @@ class ServerImpl
       current_leader,
       current_term as int,
       voted_for,
-      log,
+      AbstractifyCLogEntrySeqToRaftLogEntrySeq(log),
       commit_index as int,
       last_applied as int,
-      next_index,
-      match_index,
+      MapUint64MapValueToInt(next_index),
+      MapUint64MapValueToInt(match_index),
       num_replicated,
       app_state.Abstractify()
     )
   }
 
   function AbstractifyToRaftServerScheduler() : RaftServerScheduler
+    requires Valid()
     reads this
+    reads this.app_state
+    reads if net_client != null then NetClientIsValid.reads(net_client) else {}
   {
     RaftServerScheduler(
       this.AbstractifyToRaftServer(),
       this.nextActionIndex as int
     )
+  }
+
+  method BecomeLeader() returns ()
+    requires Valid()
+    requires MaxLogEntryIndex() - LastLogEntryIndex() as int >= 1
+    modifies this
+    ensures this.role.Leader?
+    ensures this.net_client == old(this.net_client)
+    ensures Valid()
+  {
+    var i := 0;
+    var last_log_entry := GetLastLogEntry();
+    assert log[|log| - 1].index == last_log_entry.index;
+    this.role := Candidate;
+    while i < |config.global_config.server_eps|
+      invariant 0 <= i <= |config.global_config.server_eps|
+      decreases |config.global_config.server_eps| - i
+      invariant !role.Leader?
+      invariant 1 <= |log| <= ServerMaxLogSize() as int
+      invariant log[|log| - 1] == old(log)[|old(log)| - 1]
+      invariant log[|log| - 1].index == old(log)[|old(log)| - 1].index
+      invariant forall i_ :: 0 <= i_ < i ==> (
+        var ep_ := config.global_config.server_eps[i_]; 
+        && ep_ in next_index 
+        && ep_ in match_index
+        && 1 <= next_index[ep_] <= |log| as uint64
+        && 0 <= match_index[ep_] < next_index[ep_]
+      )
+      invariant Valid()
+      invariant log == old(log)
+      invariant this.net_client == old(this.net_client)
+    {
+      var ep := config.global_config.server_eps[i];
+      next_index := next_index[ep := last_log_entry.index + 1];
+      assert last_log_entry.index >= 0;
+      assert next_index[ep] >= 1;
+      if ep != local_addr {
+        match_index := match_index[ep := 0];
+      } else {
+        match_index := match_index[ep := last_log_entry.index];
+      }
+      i := i + 1;
+    }
+    this.role := Leader;
+    assert forall ep :: ep in config.global_config.server_eps ==> ep in next_index && ep in match_index;
   }
 
   method Init(
@@ -129,13 +216,16 @@ class ServerImpl
     ghost env:HostEnvironment
   ) returns (ok:bool)
     requires env.Valid() && env.ok.ok()
+    requires nc.env == env
     requires NetClientIsValid(nc)
     requires ServerConfigStateIsValid(config)
     requires EndPoint(nc.MyPublicKey()) == config.server_ep
     requires WellFormedRaftServerConfig(AbstractifyServerConfigStateToRaftServerConfig(config))
     modifies this
-    ensures Valid()
-    ensures Env() == nc.env
+    ensures ok ==> (
+      && Valid()
+      && Env() == nc.env
+    )
   {
     this.config := config;
     this.net_client := nc;
@@ -144,11 +234,20 @@ class ServerImpl
     this.msg_grammar := CMessage_grammar();
     this.repr := { this } + NetClientRepr(net_client);
     this.current_leader := Some(this.config.global_config.server_eps[0]);
+    this.log := [CLogEntry(0, 0, [], 0, 1)];
+    this.role := Follower;
+    // TODO: Remove this
+    this.current_term := 1;
+    assert LastLogEntryIndex() == 0;
     if this.current_leader.Some? && this.config.server_ep == this.current_leader.v {
-      this.role := Leader;
+      assert MaxLogEntryIndex() - LastLogEntryIndex() as int >= 1;
+      this.BecomeLeader();
+      assert net_client.env == nc.env;
     } else{
       this.role := Follower;
+      this.current_term := 0;
     }
+    assert net_client.env == nc.env;
     ok := true;
   }
 
@@ -166,5 +265,169 @@ class ServerImpl
   {
     index := GetEndPointIndex(config.global_config, config.server_ep);
   }
+
+  function method LastLogEntryIndex() : uint64
+    requires Valid()
+    reads this
+    reads this.app_state
+    reads if net_client != null then NetClientIsValid.reads(net_client) else {}
+    requires 1 <= |log| <= ServerMaxLogSize()
+    ensures LastLogEntryIndex() as int <= MaxLogEntryIndex()
+    // TODO: this may not be true when truncating
+    ensures LastLogEntryIndex() as int == |log| - 1
+  {
+    log[|log| - 1].index
+  }
+
+  method GetLastLogEntry() returns(log_entry:CLogEntry)
+    requires Valid()
+    requires |log| - 1 >= 0
+    ensures log_entry in log
+    ensures log_entry == log[|log| - 1]
+    ensures Valid();
+  {
+    assert |log| - 1 >= 0;
+    log_entry := log[|log| - 1];
+  }
+
+  method AddLogEntries(entries:seq<CLogEntry>) returns()
+    requires Valid()
+    requires forall entry :: entry in entries ==> ValidLogEntry(entry)
+    requires |entries| <= ServerMaxLogSize() - |this.log|
+    requires LogEntrySeqIndexIncreasing(entries)
+    requires |entries| > 0 ==> (LastLogEntryIndex() + 1 == entries[0].index == |log| as uint64)
+    requires (forall i :: 0 <= i < |entries| ==> entries[i].index as int == i+|log|)
+    modifies this
+    ensures Valid()
+    ensures this.role == old(this.role)
+    ensures log == old(log) + entries
+    ensures this.Env() == old(this.Env())
+    ensures this.nextActionIndex == old(this.nextActionIndex)
+    ensures this.repr == old(this.repr)
+  {
+    this.log := this.log + entries;
+  }
+
+  method CreateLogEntry(seqno_req:uint64, req:CAppRequest) returns (ok:bool, entry:CLogEntry)
+    requires this.Valid()
+    requires 0 <= seqno_req as int <= MaxSeqno()
+    requires CAppRequestMarshallable(req)
+    ensures ok ==> (
+      && this.Valid()
+      && ValidLogEntry(entry)
+    )
+  {
+    var last_log_entry := this.GetLastLogEntry();
+    var last_log_index:uint64 := last_log_entry.index;
+    var last_log_term:uint64 := last_log_entry.term;
+
+    if last_log_index >= ServerMaxLogSize() as uint64 {
+      ok := false;
+      return;
+    }
+
+    entry := CLogEntry(this.current_term, last_log_index + 1, req, seqno_req, /*is_commited*/0);
+    ok := true;
+  }
+
+  method PrepareAppendEntriesPacket(ep:EndPoint, is_heartbeat:bool) returns (ok:bool, packet:CPacket)
+    requires this.role.Leader?
+    requires Valid()
+    requires ep in config.global_config.server_eps
+    ensures ok ==> (
+      && packet.msg.CMessage_AppendEntries?
+      && packet.dst == ep
+      && packet.src == this.config.server_ep == this.local_addr
+      && CPacketIsSendable(packet)
+      && CPacketIsAbstractable(packet)
+      && this.nextActionIndex == old(this.nextActionIndex)
+    )
+  {
+    ok := false;
+    var next_index:uint64 := this.next_index[ep];
+    var entries;
+    if is_heartbeat {
+      entries := [];
+    } else {
+      var log_index_end:uint64;
+      if |this.log| < next_index as int + LogEntrySeqSizeLimit() {
+        log_index_end := |this.log| as uint64;
+      } else {
+        log_index_end := next_index + LogEntrySeqSizeLimit() as uint64;
+      }
+      entries := this.log[next_index..log_index_end];
+      assert |entries| <= LogEntrySeqSizeLimit();
+    }
+    var prev_log_index:uint64 := next_index - 1;
+    assert prev_log_index >= 0;
+    assert prev_log_index as int < |log|;
+    var prev_log_term := log[prev_log_index].term;
+    var leader_ep := this.config.server_ep;
+
+    var last_log_entry := GetLastLogEntry();
+    print "next_index=", next_index, ", last_log_entry.index=", last_log_entry.index, "\n";
+    if next_index <= last_log_entry.index || is_heartbeat {
+      ok := true;
+      packet := CPacket(
+        ep, 
+        leader_ep, 
+        CMessage_AppendEntries(
+          this.current_term, leader_ep, prev_log_index, prev_log_term, entries, this.commit_index
+        )
+      );
+    } else {
+      ok := false;
+    }
+  }
 }
+
+
+method Server_CreateAppendEntriesForAll(server_impl:ServerImpl) returns (ok:bool, outbound_packets:seq<CPacket>)
+  requires server_impl.Valid()
+  requires server_impl.role.Leader?
+  ensures server_impl.Valid()
+  ensures server_impl.role.Leader?
+  ensures |outbound_packets| <= |server_impl.config.global_config.server_eps|
+  ensures (forall p :: p in outbound_packets ==> (
+    CPacketIsSendable(p) && CPacketIsAbstractable(p) && p.src == server_impl.config.server_ep
+  ))
+  ensures server_impl.Env() == old(server_impl.Env())
+  ensures server_impl.nextActionIndex == old(server_impl.nextActionIndex)
+  ensures server_impl.repr == old(server_impl.repr)
+  ensures ok ==> (
+    && OutboundPacketsIsValid(PacketSequence(outbound_packets))
+  )
+{
+  outbound_packets := [];
+  var i := 0;
+  while i < |server_impl.config.global_config.server_eps|
+    decreases |server_impl.config.global_config.server_eps| - i
+    invariant server_impl.Valid()
+    invariant 0 <= i <= |server_impl.config.global_config.server_eps|
+    invariant server_impl.role.Leader?
+    invariant |outbound_packets| <= i
+    invariant |outbound_packets| <= |server_impl.config.global_config.server_eps|
+    invariant (forall p :: p in outbound_packets ==> (
+      CPacketIsSendable(p) && CPacketIsAbstractable(p) && p.src == server_impl.config.server_ep
+    ))
+    invariant server_impl.Env() == old(server_impl.Env())
+    invariant server_impl.nextActionIndex == old(server_impl.nextActionIndex)
+    invariant server_impl.repr == old(server_impl.repr)
+  {
+    var ep := server_impl.config.global_config.server_eps[i];
+    if ep != server_impl.config.server_ep {
+      var packet;
+      ok, packet := server_impl.PrepareAppendEntriesPacket(ep, false);
+      if (!ok) {
+        break;
+      }
+      print "ready to send to ", i, " with AppendEntries(", |packet.msg.entries|, ")\n";
+      assert CPacketIsSendable(packet);
+      outbound_packets := outbound_packets + [packet];
+    }
+    i := i + 1;
+    assert |outbound_packets| <= i;
+  }
+}
+
 }
