ironfleet/src/Dafny/Distributed/Impl/Raft/ServerImplProcessPacketX.i.dfy
@@ -4,6 +4,8 @@ include "../../../Libraries/Math/mod_auto.i.dfy"
 include "../../Protocol/Raft/Server.i.dfy"
 include "../../Protocol/Raft/Types.i.dfy"
 include "../Common/UpperBound.i.dfy"
+include "AppInterface.i.dfy"
+include "CBroadcast.i.dfy"
 include "CMessage.i.dfy"
 include "Config.i.dfy"
 include "CTypes.i.dfy"
@@ -24,6 +26,8 @@ import opened Math__mod_auto_i
 import opened Common__NetClient_i
 import opened Common__UpperBound_i
 import opened Environment_s
+import opened Raft__AppInterface_i
+import opened Raft__CBroadcast_i
 import opened Raft__ConfigState_i
 import opened Raft__CTypes_i
 import opened Raft__CMessage_i
@@ -34,6 +38,330 @@ import opened Raft__ServerImpl_i
 import opened Raft__Types_i
 import opened Raft__ServerImplDelivery_i
 
+//////////////////////////////////////////////////////////
+// Process request from client
+//////////////////////////////////////////////////////////
+method Server_Next_ProcessRequest(server_impl:ServerImpl, ghost old_net_history:seq<NetEvent>, rr:ReceiveResult, ghost receive_event:NetEvent)
+  returns (ok:bool, ghost net_event_log:seq<NetEvent>, ghost ios:seq<RaftIo>)
+  requires receive_event.LIoOpReceive?
+  requires rr.RRPacket?
+  requires NetPacketIsAbstractable(receive_event.r)
+  requires rr.cpacket.msg.CMessage_Request?
+  requires server_impl.Valid()
+  requires server_impl.Env().net.history() == old_net_history + [receive_event]
+  requires CPacketIsSendable(rr.cpacket)
+  requires ConfigStateIsValid(server_impl.config.global_config)
+  modifies server_impl, server_impl.repr, server_impl.net_client;
+  ensures server_impl.repr == old(server_impl.repr)
+  ensures server_impl.net_client != null
+  ensures server_impl.Env().Valid() && server_impl.Env().ok.ok() ==> ok
+  ensures server_impl.Env() == old(server_impl.Env());
+  ensures ok ==> 
+            && server_impl.Valid()
+            && server_impl.nextActionIndex == old(server_impl.nextActionIndex)
+            // PROVE
+            // && (|| Q_RaftServer_Next_ProcessPacket(old(server_impl.AbstractifyToRaftServer()), server_impl.AbstractifyToRaftServer(), ios)
+            //     || (&& IosReflectIgnoringUnsendable(net_event_log)
+            //        && old(server_impl.AbstractifyToRaftServer()) == server_impl.AbstractifyToRaftServer()))
+            && RawIoConsistentWithSpecIO(net_event_log, ios)
+            && OnlySentMarshallableData(net_event_log)
+            && old_net_history + net_event_log == server_impl.Env().net.history()
+            && forall i :: 0 <= i < |net_event_log| - 1 ==> net_event_log[i].LIoOpReceive? || net_event_log[i+1].LIoOpSend?
+{
+  ok := true;
+  ghost var receive_io := LIoOpReceive(AbstractifyNetPacketToRaftPacket(receive_event.r));
+  var recved_msg := rr.cpacket.msg;
+  ghost var ios_head := [receive_io];
+  ghost var log_head := [receive_event];
+  ghost var log_tail := [];                                                                                                                                                                                                                                                                                                                                                                                                                                                                                                                                                                                                                                                                                                                                                                                                                                                                                                      
+  ghost var ios_tail := [];
+  net_event_log := log_head;
+  ios := ios_head;
+  ok := true;
+  
+  if server_impl.role == Leader {
+    var leader_ep := server_impl.config.server_ep;
+    var leader_id := GetEndPointIndex(server_impl.config.global_config, leader_ep);
+    // create entry
+    var entry;
+    print "trying to create log\n";
+    ok, entry := server_impl.CreateLogEntry(recved_msg.seqno_req, recved_msg.req);
+    print "created log: ", ok, "\n";
+    if (!ok) {
+      ok := true;
+      return;
+    }
+    // Append entry to leader's log
+    if (
+      1 > ServerMaxLogSize() - |server_impl.log| 
+      || !(server_impl.LastLogEntryIndex() + 1 == entry.index == |server_impl.log| as uint64)
+    ) {
+      print "append failed!!!",server_impl.LastLogEntryIndex() + 1, ",", entry.index, ",", |server_impl.log| as uint64, "\n";
+      ok := true;
+      return;
+    }
+    server_impl.AddLogEntries([entry]);
+    server_impl.next_index := server_impl.next_index[leader_ep := entry.index + 1];
+    server_impl.match_index := server_impl.match_index[leader_ep := entry.index];
+    assert server_impl.role.Leader?;
+    print "append success!!!\n";
+    // Create packets
+    var outbound_packets:seq<CPacket> := [];
+    ok, outbound_packets := Server_CreateAppendEntriesForAll(server_impl);
+    if (!ok) {
+      ok := true;
+      return;
+    }
+    assert |outbound_packets| <= |server_impl.config.global_config.server_eps| <= 0xFFFF_FFFF_FFFF_FFFF;
+    assert (forall p :: p in outbound_packets ==> CPacketIsSendable(p));
+    ok, log_tail, ios_tail := DeliverOutboundPackets(server_impl, PacketSequence(outbound_packets));
+    if (!ok) { return; }
+    ios := ios_head + ios_tail;
+    net_event_log := log_head + log_tail;
+    assert net_event_log[0].LIoOpReceive?;
+    assert forall i::0<=i<|log_tail| ==> AbstractifyNetEventToRaftIo(log_tail[i]) == ios_tail[i];
+    assert forall i::0<=i<|log_tail| ==> log_tail[i].LIoOpSend? && ios_tail[i].LIoOpSend?;
+    assert forall i :: 1 <= i < |net_event_log| ==> net_event_log[i].LIoOpSend?;
+    assert forall i :: 0 <= i < |net_event_log| - 1 ==> net_event_log[i].LIoOpReceive? || net_event_log[i+1].LIoOpSend?;
+  } else {
+    var leader_id;
+    if (server_impl.current_leader.Some?) {
+      leader_id := GetEndPointIndex(server_impl.config.global_config, server_impl.current_leader.v);
+    } else {
+      leader_id := GetEndPointIndex(server_impl.config.global_config, server_impl.config.server_ep);
+    }
+    var msg := CMessage_Reply(recved_msg.seqno_req, 1, leader_id, []);
+    var packet := CPacket(rr.cpacket.src, server_impl.config.server_ep , msg);
+    var outbound_packets := OutboundPacket(Some(packet));
+    ok, log_tail, ios_tail := DeliverOutboundPackets(server_impl, outbound_packets);
+    if (!ok) { return; }
+    ios := ios_head + ios_tail;
+    net_event_log := log_head + log_tail;
+    assert net_event_log[0].LIoOpReceive?;
+    assert forall i::0<=i<|log_tail| ==> AbstractifyNetEventToRaftIo(log_tail[i]) == ios_tail[i];
+    assert forall i::0<=i<|log_tail| ==> log_tail[i].LIoOpSend? && ios_tail[i].LIoOpSend?;
+    assert forall i :: 1 <= i < |net_event_log| ==> net_event_log[i].LIoOpSend?;
+    assert forall i :: 0 <= i < |net_event_log| - 1 ==> net_event_log[i].LIoOpReceive? || net_event_log[i+1].LIoOpSend?;
+  }
+}
+
+//////////////////////////////////////////////////////////
+// Process AppendEntries
+//////////////////////////////////////////////////////////
+method Server_ResetNextElectionTime(server_impl:ServerImpl) returns (ghost clock_event:NetEvent, ghost clock_io:RaftIo)
+  requires server_impl.role == Follower
+  requires server_impl.Valid()
+  // requires history_after_recv == server_impl.Env().net.history()
+  modifies server_impl, NetClientRepr(server_impl.net_client)
+  ensures clock_event.LIoOpReadClock? && clock_io.LIoOpReadClock?
+  ensures server_impl.role == Follower
+  ensures server_impl.Valid()
+  // ensures io and event consistent
+  ensures AbstractifyNetEventToRaftIo(clock_event) == clock_io
+  // ensures history correctly changed
+  ensures old(server_impl.Env().net.history()) + [clock_event] == server_impl.Env().net.history()
+  // make sure some fields unchanged
+  ensures server_impl.repr == old(server_impl.repr)
+  ensures server_impl.Env() == old(server_impl.Env())
+  ensures server_impl.nextActionIndex == old(server_impl.nextActionIndex)
+  ensures RawIoConsistentWithSpecIO([clock_event], [clock_io])
+  ensures server_impl.log == old(server_impl.log)
+{
+  var const_params := server_impl.config.global_config.params;
+  var clock;
+  clock, clock_event := ReadClock(server_impl.net_client);
+  var election_timeout_delta := GenerateElectionTimeout(const_params);
+  var next_election_time := UpperBoundedAdditionImpl(clock.t, election_timeout_delta, const_params.max_integer_value);
+  server_impl.next_election_time := next_election_time;
+  clock_io := LIoOpReadClock(clock.t as int);
+}
+
+method Server_HandleAppendEntries(server_impl:ServerImpl, ghost old_net_history:seq<NetEvent>, rr:ReceiveResult, ghost receive_event:NetEvent) 
+  returns (ok:bool, ghost net_event_log:seq<NetEvent>, ghost ios:seq<RaftIo>)
+  // About recved things
+  requires receive_event.LIoOpReceive?
+  requires rr.RRPacket?
+  requires NetPacketIsAbstractable(receive_event.r)
+  requires rr.cpacket.msg.CMessage_AppendEntries?
+  // About server
+  requires server_impl.Valid()
+  requires server_impl.Env().net.history() == old_net_history + [receive_event]
+  requires CPacketIsSendable(rr.cpacket)
+  requires ConfigStateIsValid(server_impl.config.global_config)
+  modifies server_impl, server_impl.repr, server_impl.net_client;
+  ensures server_impl.repr == old(server_impl.repr)
+  ensures server_impl.net_client != null
+  ensures server_impl.Env().Valid() && server_impl.Env().ok.ok() ==> ok
+  ensures server_impl.Env() == old(server_impl.Env());
+  ensures ok ==> 
+            && server_impl.Valid()
+            && server_impl.nextActionIndex == old(server_impl.nextActionIndex)
+            // PROVE
+            // && (|| Q_RaftServer_Next_ProcessPacket(old(server_impl.AbstractifyToRaftServer()), server_impl.AbstractifyToRaftServer(), ios)
+            //     || (&& IosReflectIgnoringUnsendable(net_event_log)
+            //        && old(server_impl.AbstractifyToRaftServer()) == server_impl.AbstractifyToRaftServer()))
+            && RawIoConsistentWithSpecIO(net_event_log, ios)
+            && OnlySentMarshallableData(net_event_log)
+            && old_net_history + net_event_log == server_impl.Env().net.history()
+            && forall i :: 0 <= i < |net_event_log| - 1 ==> net_event_log[i].LIoOpReceive? || net_event_log[i+1].LIoOpSend?
+{
+  ghost var receive_io := LIoOpReceive(AbstractifyNetPacketToRaftPacket(receive_event.r));
+  var msg := rr.cpacket.msg;
+
+  var success := 0;
+  var match_index := 0;
+  if (server_impl.current_term < msg.term) {
+    server_impl.current_term := msg.term;
+    server_impl.voted_for := None;
+    server_impl.role := Follower;
+  }
+  var my_last_log := server_impl.GetLastLogEntry();
+  assert server_impl.Valid();
+  if (server_impl.current_term == msg.term) {
+    print "Trying to append #of entries=", |msg.entries|, "\n";
+    // Reset role to follower;
+    server_impl.role := Follower;
+    // And reset Election Timeout
+    ghost var clock_event, clock_io := Server_ResetNextElectionTime(server_impl);
+    assert my_last_log.index as int == |server_impl.log| - 1;
+    assert server_impl.Valid();
+    net_event_log := [receive_event, clock_event];
+    ios := [receive_io, clock_io];
+    assert net_event_log[0].LIoOpReceive?;
+    assert net_event_log[1].LIoOpReadClock?;
+    // check whether we can put the entries
+    if msg.prev_log_index > 0xFFFF_FFFF_FFFF_FFFE 
+      && (msg.prev_log_index as int + 1 + |msg.entries| > ServerMaxLogSize()
+    ){
+      ok := true;
+      print "[Error] msg.prev_log_index too large";
+      return;
+    }
+    if (msg.prev_log_index == 0 
+      || (msg.prev_log_index <= my_last_log.index && msg.prev_log_term == my_last_log.term)
+    ) {
+      success := 1;
+      assert |msg.entries| > 0 ==> server_impl.log[msg.prev_log_index].index as int + 1 == msg.entries[0].index as int;
+      server_impl.log := server_impl.log[..msg.prev_log_index+1] + msg.entries;
+      if |msg.entries| == 0 {
+        match_index := msg.prev_log_index;
+      } else {
+        match_index := my_last_log.index;
+      }
+      if (msg.leader_commit > server_impl.commit_index) {
+        server_impl.commit_index := msg.leader_commit;
+      }
+      print "After appending, |log|=", |server_impl.log|, "\n";
+    } else {
+      print "Not yet uptodate, cannot append\n";
+    }
+    var send_msg := CMessage_AppendEntriesReply(server_impl.current_term, success, match_index);
+    var send_packet := CPacket(rr.cpacket.src, server_impl.config.server_ep, send_msg);
+    ghost var log_tail, ios_tail;
+    ok, log_tail, ios_tail := DeliverOutboundPackets(server_impl, OutboundPacket(Some(send_packet)));
+    if (!ok) { return; }
+    net_event_log := net_event_log + log_tail;
+    ios := ios + ios_tail;
+    assert forall i::0<=i<|log_tail| ==> AbstractifyNetEventToRaftIo(log_tail[i]) == ios_tail[i];
+    assert forall i::0<=i<|log_tail| ==> log_tail[i].LIoOpSend? && ios_tail[i].LIoOpSend?;
+    assert forall i :: 0 <= i < |net_event_log| - 1 ==> net_event_log[i].LIoOpReceive? || net_event_log[i+1].LIoOpSend?;
+  } else {
+    net_event_log := [receive_event];
+    ios := [receive_io];
+    ok := true;
+  }
+}
+
+//////////////////////////////////////////////////////////
+// Process AppendEntriesReply
+//////////////////////////////////////////////////////////
+method Server_HandleAppendEntriesReply(server_impl:ServerImpl, ghost old_net_history:seq<NetEvent>, rr:ReceiveResult, ghost receive_event:NetEvent) 
+  returns (ok:bool, ghost net_event_log:seq<NetEvent>, ghost ios:seq<RaftIo>)
+  // About recved things
+  requires receive_event.LIoOpReceive?
+  requires rr.RRPacket?
+  requires NetPacketIsAbstractable(receive_event.r)
+  requires rr.cpacket.msg.CMessage_AppendEntriesReply?
+  // About server
+  requires server_impl.role == Leader
+  requires server_impl.Valid()
+  requires server_impl.Env().net.history() == old_net_history + [receive_event]
+  requires CPacketIsSendable(rr.cpacket)
+  requires ConfigStateIsValid(server_impl.config.global_config)
+  modifies server_impl, server_impl.repr, server_impl.net_client;
+  ensures server_impl.repr == old(server_impl.repr)
+  ensures server_impl.net_client != null
+  ensures server_impl.Env().Valid() && server_impl.Env().ok.ok() ==> ok
+  ensures server_impl.Env() == old(server_impl.Env());
+  ensures ok ==> 
+            && server_impl.Valid()
+            && server_impl.nextActionIndex == old(server_impl.nextActionIndex)
+            // PROVE
+            // && (|| Q_RaftServer_Next_ProcessPacket(old(server_impl.AbstractifyToRaftServer()), server_impl.AbstractifyToRaftServer(), ios)
+            //     || (&& IosReflectIgnoringUnsendable(net_event_log)
+            //        && old(server_impl.AbstractifyToRaftServer()) == server_impl.AbstractifyToRaftServer()))
+            && RawIoConsistentWithSpecIO(net_event_log, ios)
+            && OnlySentMarshallableData(net_event_log)
+            && old_net_history + net_event_log == server_impl.Env().net.history()
+            && forall i :: 0 <= i < |net_event_log| - 1 ==> net_event_log[i].LIoOpReceive? || net_event_log[i+1].LIoOpSend?
+{
+  ghost var receive_io := LIoOpReceive(AbstractifyNetPacketToRaftPacket(receive_event.r));
+  var msg := rr.cpacket.msg;
+  // setup default return values
+  net_event_log := [receive_event];
+  ios := [receive_io];
+  ok := true;
+
+  // Check and update term
+  if (server_impl.current_term < msg.term) {
+    server_impl.current_term := msg.term;
+    server_impl.voted_for := None;
+    server_impl.role := Follower;
+    return;
+  }
+  
+  var ep := rr.cpacket.src;
+  if (ep !in server_impl.config.global_config.server_eps) {
+    print "[Error] src of the packet not in cluster\n";
+    return;
+  }
+
+  if (server_impl.role == Leader && server_impl.current_term == msg.term) {
+    if (msg.success == 1) {
+      assert forall ep :: ep in server_impl.config.global_config.server_eps ==> (
+        && ep in server_impl.next_index 
+        && ep in server_impl.match_index
+        && 1 <= server_impl.next_index[ep] <= |server_impl.log| as uint64
+        && 0 <= server_impl.match_index[ep] < server_impl.next_index[ep]
+      );
+      if (msg.match_index > MaxLogEntryIndex() as uint64 - 1) {
+        print "[Error] match_index too large\n";
+        return;
+      }
+      if (msg.match_index + 1 > |server_impl.log| as uint64) {
+        print "[Error] should not be\n";
+        return;
+      }
+      if (msg.match_index > server_impl.match_index[ep]) {
+        server_impl.match_index := server_impl.match_index[ep := msg.match_index];
+      }
+      server_impl.next_index := server_impl.next_index[ep := server_impl.match_index[ep] + 1];
+    } else {
+      var decreased_index;
+      if server_impl.next_index[ep] > 1 {
+        decreased_index := server_impl.next_index[ep];
+      } else {
+        decreased_index := 1;
+      }
+      server_impl.next_index := server_impl.next_index[ep := decreased_index];
+    }
+  }
+
+}
+
+//////////////////////////////////////////////////////////
+// Process All Packet.
+//////////////////////////////////////////////////////////
 method Server_Next_ProcessPacketX(server_impl:ServerImpl)
   returns (ok:bool, ghost net_event_log:seq<NetEvent>, ghost ios:seq<RaftIo>)
   requires server_impl.Valid()
@@ -41,7 +369,6 @@ method Server_Next_ProcessPacketX(server_impl:ServerImpl)
   modifies server_impl, server_impl.repr, server_impl.net_client;
   ensures server_impl.repr == old(server_impl.repr)
   ensures server_impl.net_client != null
-  ensures ok == NetClientOk(server_impl.net_client)
   ensures server_impl.Env().Valid() && server_impl.Env().ok.ok() ==> ok
   ensures server_impl.Env() == old(server_impl.Env());
   ensures ok ==> 
@@ -60,6 +387,8 @@ method Server_Next_ProcessPacketX(server_impl:ServerImpl)
 
   var rr, receive_event := Receive(server_impl.net_client, server_impl.config.server_ep, server_impl.config.global_config, server_impl.msg_grammar);
   
+  assert server_impl.Env()==old(server_impl.Env());
+
   if (rr.RRFail?) {
     ok := false;
     net_event_log := [];
@@ -71,82 +400,42 @@ method Server_Next_ProcessPacketX(server_impl:ServerImpl)
     ios := [LIoOpTimeoutReceive()];
   } else {
     var marshallable := DetermineIfMessageMarshallable(rr.cpacket.msg);
+    ghost var receive_io := LIoOpReceive(AbstractifyNetPacketToRaftPacket(receive_event.r));
+    // setup default return
+    net_event_log := [receive_event];
+    ios := [receive_io];
+    ok := true;
     if !marshallable {
-      ok := true;
-      ghost var receive_io := LIoOpReceive(AbstractifyNetPacketToRaftPacket(receive_event.r));
-      net_event_log := [receive_event];
-      ios := [receive_io];
-    } else if (rr.cpacket.msg.CMessage_AppendEntries?) {
-      ok := true;
-      var const_params := server_impl.config.global_config.params;
-      var clock, clock_event := ReadClock(server_impl.net_client);
-      var election_timeout_delta := GenerateElectionTimeout(const_params);
-      var next_election_time := UpperBoundedAdditionImpl(clock.t, election_timeout_delta, const_params.max_integer_value);
-      server_impl.next_election_time := next_election_time;
-      ghost var receive_io := LIoOpReceive(AbstractifyNetPacketToRaftPacket(receive_event.r));
-      ghost var clock_io := LIoOpReadClock(clock.t as int);
-      net_event_log := [receive_event, clock_event];
-      ios := [receive_io, clock_io];
-      assert net_event_log[0].LIoOpReceive?;
-      assert net_event_log[1].LIoOpReadClock?;
-    } else {
-      ok := true;
-      ghost var receive_io := LIoOpReceive(AbstractifyNetPacketToRaftPacket(receive_event.r));
-      var my_idx := server_impl.GetMyIndex();
-      print my_idx, " received a request1", rr.cpacket.msg, ", marshallable=", marshallable, "\n";
-      if (rr.cpacket.msg.CMessage_Invalid?) {
-        ok := true;
-        net_event_log := [receive_event];
-        ios := [receive_io];
-      } else if (rr.cpacket.msg.CMessage_Request?) {
-        ok := true;
-        var recved_msg := rr.cpacket.msg;
-        ghost var ios_head := [receive_io];
-        ghost var log_head := [receive_event];
-        ghost var log_tail, ios_tail;
-        if server_impl.role == Leader {
-          var leader_id;
-          if (server_impl.current_leader.Some?) {
-            leader_id := GetEndPointIndex(server_impl.config.global_config, server_impl.current_leader.v);
-          } else {
-            leader_id := GetEndPointIndex(server_impl.config.global_config, server_impl.config.server_ep);
-          }
-          var msg := CMessage_Reply(recved_msg.seqno_req, 1, leader_id, []);
-          var packet := CPacket(rr.cpacket.src, server_impl.config.server_ep , msg);
-          var outbound_packets := OutboundPacket(Some(packet));
-          ok, log_tail, ios_tail := DeliverOutboundPackets(server_impl, outbound_packets);
-          if (!ok) { return; }
-          ios := ios_head + ios_tail;
-          net_event_log := log_head + log_tail;
-          assert net_event_log[0].LIoOpReceive?;
-          assert forall i::0<=i<|log_tail| ==> AbstractifyNetEventToRaftIo(log_tail[i]) == ios_tail[i];
-          assert forall i::0<=i<|log_tail| ==> log_tail[i].LIoOpSend? && ios_tail[i].LIoOpSend?;
-          assert forall i :: 1 <= i < |net_event_log| ==> net_event_log[i].LIoOpSend?;
-          assert forall i :: 0 <= i < |net_event_log| - 1 ==> net_event_log[i].LIoOpReceive? || net_event_log[i+1].LIoOpSend?;
-        } else {
-          var leader_id;
-          if (server_impl.current_leader.Some?) {
-            leader_id := GetEndPointIndex(server_impl.config.global_config, server_impl.current_leader.v);
-          } else {
-            leader_id := GetEndPointIndex(server_impl.config.global_config, server_impl.config.server_ep);
-          }
-          var msg := CMessage_Reply(recved_msg.seqno_req, 1, leader_id, []);
-          var packet := CPacket(rr.cpacket.src, server_impl.config.server_ep , msg);
-          var outbound_packets := OutboundPacket(Some(packet));
-          ok, log_tail, ios_tail := DeliverOutboundPackets(server_impl, outbound_packets);
-          if (!ok) { return; }
-          ios := ios_head + ios_tail;
-          net_event_log := log_head + log_tail;
-          assert net_event_log[0].LIoOpReceive?;
-          assert forall i::0<=i<|log_tail| ==> AbstractifyNetEventToRaftIo(log_tail[i]) == ios_tail[i];
-          assert forall i::0<=i<|log_tail| ==> log_tail[i].LIoOpSend? && ios_tail[i].LIoOpSend?;
-          assert forall i :: 1 <= i < |net_event_log| ==> net_event_log[i].LIoOpSend?;
-          assert forall i :: 0 <= i < |net_event_log| - 1 ==> net_event_log[i].LIoOpReceive? || net_event_log[i+1].LIoOpSend?;
-        }
+      return;
+    }
+    var my_idx := server_impl.GetMyIndex();
+    var msg := rr.cpacket.msg;
+    if (msg.CMessage_Request? || msg.CMessage_Reply?) {
+      if (msg.CMessage_Request?) {
+        print "server ", my_idx, "(is_leader=", server_impl.role.Leader?, ") received a request(", msg.seqno_req, ", ", msg.req, ")\n";
+        ok, net_event_log, ios := Server_Next_ProcessRequest(server_impl, old_net_history, rr, receive_event);
       } else {
-        ok := true;
-        net_event_log := [receive_event];
-        ios := [receive_io];
+        return;
+      }
+    } else {
+      assert msg.CMessage_AppendEntries? || msg.CMessage_AppendEntriesReply? || msg.CMessage_RequestVote? || msg.CMessage_RequestVoteReply?;
+      if (msg.CMessage_AppendEntries?) {
+        // ignore packet from self
+        if (rr.cpacket.src == server_impl.config.server_ep) {
+          return;
+        }
+        print "server ", my_idx, "(is_leader=", server_impl.role.Leader?, 
+          ") received AppendEntries(|entries|=", |msg.entries|, ",prev_log_index=", msg.prev_log_index, ")\n";
+        ok, net_event_log, ios := Server_HandleAppendEntries(server_impl, old_net_history, rr, receive_event);
+      } else if (msg.CMessage_AppendEntriesReply?) {
+        if (server_impl.role != Leader) {
+          return;
+        }
+        print "server ", my_idx, "(is_leader=", server_impl.role.Leader?, 
+          ") received AppendEntriesReply(term=", msg.term, ",success=", msg.success, "match_index=", msg.match_index, ")\n";
+        ok, net_event_log, ios := Server_HandleAppendEntriesReply(server_impl, old_net_history, rr, receive_event);
+      } else {
+        return;
       }
     }
   }
